plugins/Types/LTS/edu.toronto.cs.se.mmint.types.lts.operators/lean/property_catalogue/LTL/pattern_meta.lean
@@ -4,10 +4,22 @@ import proof_state tactic
 
 variable {α : Type}
 
-meta def switch (ps : PROOF_STATE α) : tactic (PROOF_STATE α) := 
+def is_even (n : ℕ) : Prop := ∃ k : ℕ, 2 * k = n 
+
+lemma double_even : ∀ n : ℕ, is_even (2 * n)  := 
+  λ n, Exists.intro n (rfl)
+
+theorem four_is_even : is_even 14 := 
+begin
+  apply double_even 7, 
+end 
+
+
+meta def switch (ps : proofState α) : tactic (proofState α) := 
 do 
   tgt ← tactic.target, ctx ← tactic.local_context,
   match tgt with
+  -- need to update 
   -- | `(sat (precedes.globally %%e₁ %%e₂) _) :=  
   --   precedes.globally.solve e₁ e₂ ps ctx
   | `(sat (absent.globally %%e₁) _) :=  do 
