plugins/Types/LTS/edu.toronto.cs.se.mmint.types.lts.operators/lean/LTS/default.lean
@@ -1,1 +1,0 @@
-import LTS.defs 
