plugins/Types/LTS/edu.toronto.cs.se.mmint.types.lts.operators/lean/property_catalogue/LTL/default.lean
@@ -1,4 +1,4 @@
-import LTS 
+import LTS.defs
 import property_catalogue.LTL.patterns
 import property_catalogue.LTL.pattern_meta
 import property_catalogue.LTL.sat.absent 
