plugins/Types/LTS/edu.toronto.cs.se.mmint.types.lts.operators/lean/property_catalogue/LTL/sat/precedes.lean
@@ -1,4 +1,4 @@
-import LTS property_catalogue.LTL.patterns tactic
+import LTS.defs property_catalogue.LTL.patterns tactic
 
 open tactic
 
